Std.lean
@@ -5,6 +5,7 @@ import Std.Data.Array.Basic
 import Std.Data.Array.Init.Basic
 import Std.Data.Array.Init.Lemmas
 import Std.Data.Array.Lemmas
+import Std.Data.AssocList
 import Std.Data.BinomialHeap
 import Std.Data.DList
 import Std.Data.Int.Basic
