Std/Data/Option/Init/Lemmas.lean
@@ -15,3 +15,9 @@ New theorems should be added to `Std.Data.Option.Lemmas` if they are not needed 
 
 @[simp] theorem getD_none : getD none a = a := rfl
 @[simp] theorem getD_some : getD (some a) b = a := rfl
+
+@[simp] theorem map_none' (f : α → β) : none.map f = none := rfl
+@[simp] theorem map_some' (a) (f : α → β) : (some a).map f = some (f a) := rfl
+
+@[simp] theorem none_bind (f : α → Option β) : none.bind f = none := rfl
+@[simp] theorem some_bind (a) (f : α → Option β) : (some a).bind f = f a := rfl
